ver2/checker.v
@@ -135,7 +135,7 @@ destruct instr eqn: eq_instr.
   simpl in Hsymb_exec_instr.
   unfold pushtag_s in Hsymb_exec_instr.
   destruct (add_to_smap (get_smap_sst (SymExState instk_height sstk smem sstg 
-    sctx sm)) (SymPUSHTAG type v)).
+    sctx sm)) (SymMETAPUSH cat v)).
   destruct (misc.Misc.push (FreshVar n) (get_stack_sst (SymExState instk_height
     sstk smem sstg sctx sm))); try discriminate.
   injection Hsymb_exec_instr as eq_sst'. rewrite <- eq_sst'. simpl. reflexivity.
